fix

LeanYjs/Network/StrongCausalOrder.lean
@@ -3,6 +3,7 @@ import Mathlib.Order.Defs.PartialOrder
 import Mathlib.Tactic.ApplyAt
 import Mathlib.Tactic.Use
 import Mathlib.Tactic.CongrExclamation
+import Mathlib.Data.List.Induction
 
 import LeanYjs.ListLemmas
 
@@ -10,30 +11,9 @@ open List
 
 abbrev CausalOrder A := PartialOrder A
 
-section CausalOrder
-
-class WithId (A : Type) (S : outParam Type) [DecidableEq S] where
-  id : A → S
-
-class Operation (A : Type) (S : outParam Type) [DecidableEq S] [WithId A S] where
-  State : Type
-  Error : Type
-  init : State
-  effect : A → State → Except Error State
-  isValidState : A → State → Prop
-  -- TODO: is this enough to strong assumption for yjs?
-  isValidState_mono : ∀ {l₁ l₂ : List A},
-    l₁ ⊆ l₂ →
-    List.Pairwise (fun a b => WithId.id a ≠ WithId.id b) l₁ →
-    List.Pairwise (fun a b => WithId.id a ≠ WithId.id b) l₂ →
-    l₁.foldr (fun a f => fun s => effect a s >>= f) (fun a => return a) init = Except.ok s₁ →
-    l₂.foldr (fun a f => fun s => effect a s >>= f) (fun a => return a) init = Except.ok s₂ →
-    isValidState a s₁ →
-    isValidState a s₂
+section hb_concurrent
 
 variable {A : Type} [DecidableEq A] (hb : CausalOrder A)
-
-section hb_concurrent
 
 def hb_concurrent (a b : A) : Prop :=
   ¬ (hb.le a b) ∧ ¬ (hb.le b a)
@@ -94,14 +74,38 @@ omit [DecidableEq A] in lemma hb_consistent_tail (a : A) (ops : List A) :
   cases h_consistent
   assumption
 
-end hb_concurrent
-
 def hbClosed (ops : List A) : Prop :=
   ∀a b l₁ l₂, ops = l₁ ++ a :: l₂ → b < a → b ∈ l₁
 
+end hb_concurrent
+
 section effect
 
-variable [Operation A]
+class WithId (A : Type) (S : outParam Type) [DecidableEq S] where
+  id : A → S
+
+def IdNoDup {A : Type} {S : Type} [DecidableEq S] [WithId A S] (ops : List A) : Prop :=
+  List.Pairwise (fun a b => WithId.id a ≠ WithId.id b) ops
+
+class Operation (A : Type) where
+  State : Type
+  Error : Type
+  init : State
+  effect : A → State → Except Error State
+  isValidState : A → State → Prop
+
+class MonotoneOperation (A : Type) [hb : CausalOrder A] (S : outParam Type) [DecidableEq S] [WithId A S] [Operation A] extends Operation A where
+  -- TODO: is this enough to strong assumption for yjs?
+  isValidState_mono : ∀ {l : List A},
+    (∀x < a, x ∈ l) →
+    hb_consistent hb l →
+    hbClosed hb l →
+    l.foldl (fun s op => s >>= effect op) (Except.ok init) = Except.ok s →
+    IdNoDup l →
+    isValidState a s
+
+variable {A : Type} {S : Type} [DecidableEq S] {hb : CausalOrder A}
+variable [WithId A S]  [Operation A]
 
 abbrev Effect := Operation.State A → Except (Operation.Error A) (Operation.State A)
 
@@ -110,24 +114,28 @@ def effect (op : A) : Effect (A := A) :=
 
 def effect_comp (op1 op2 : Effect (A := A)) : Effect (A := A) := fun s => op1 s >>= op2
 
-local infix:99 " ▷ " => effect_comp
-
-omit [DecidableEq A] in theorem effect_comp_assoc (op1 op2 op3 : Effect (A := A)) :
+theorem effect_comp_assoc (op1 op2 op3 : Effect (A := A)) :
   effect_comp (effect_comp op1 op2) op3 = effect_comp op1 (effect_comp op2 op3) := by
   funext s
   simp [effect_comp]
   unfold effect_comp
   simp
-
 end effect
 
-def concurrent_commutative [Operation A] (list : List A) : Prop :=
-  ∀ a b (s : Operation.State A), a ∈ list → b ∈ list → hb_concurrent hb a b →
-      Operation.isValidState a s →
-      Operation.isValidState b s →
-      effect_comp (effect a) (effect b) s = effect_comp (effect b) (effect a) s
+local infix:99 " ▷ " => effect_comp
 
-omit [DecidableEq A] in theorem hb_consistent_concurrent (a : A) (ops₀ ops₁ : List A) :
+section commutativity
+
+variable {A : Type} {S : Type} [DecidableEq S] {hb : CausalOrder A}
+variable [WithId A S]  [Operation A]
+
+def concurrent_commutative (list : List A) : Prop :=
+  ∀ a b (s s' : Operation.State A), a ∈ list → b ∈ list → hb_concurrent hb a b →
+    Operation.isValidState a s →
+    Operation.isValidState b s →
+    (effect a s >>= effect b) = Except.ok s' → (effect b s >>= effect a) = Except.ok s'
+
+theorem hb_consistent_concurrent (a : A) (ops₀ ops₁ : List A) :
   hb_consistent hb (ops₀ ++ a :: ops₁) →
   ∀ x, x ∈ ops₀ → ¬a ≤ x := by
   intro h_consistent x h_mem
@@ -147,241 +155,308 @@ omit [DecidableEq A] in theorem hb_consistent_concurrent (a : A) (ops₀ ops₁ 
       | inr h_mem_tail =>
         apply ih h_consistent_tail h_mem_tail
 
-inductive compatibleOps [DecidableEq A] (hb : CausalOrder A) : Operation.State A → List A → Prop where
-  | nil : compatibleOps hb s []
-  | cons :
-      compatibleOp hb s a →
-      effect a s = Except.ok s' →
-      compatibleOps hb s' ops' →
-      compatibleOps hb s (a :: ops')
+theorem Except.bind_eq_ok_exist {α β : Type} {e : Except α β} {f : β → Except α β'} {v : β'} :
+  e >>= f = Except.ok v →
+  ∃ u : β, e = Except.ok u ∧ f u = Except.ok v := by
+  intros h
+  cases e with
+  | error err =>
+    simp [bind, Except.bind] at *
+  | ok u =>
+    refine ⟨ u, by rfl, ?_ ⟩
+    assumption
 
-theorem hb_concurrent_foldr {ops₀ ops₁ : List A} {s : Operation.State A} :
-  concurrent_commutative hb (ops₀ ++ a :: ops₁) →
-  (∀ x ∈ ops₀, hb_concurrent hb x a) →
-  compatibleOps hb s (ops₀ ++ a :: ops₁) →
-  List.foldr (effect_comp (A := A)) (effect a ▷ init) (List.map (fun a => effect a) ops₀) s =
-  (effect a ▷ List.foldr (effect_comp (A := A)) init (List.map (fun a => effect a) ops₀)) s := by
+def effect_list (ops : List A) (s : Except (Operation.Error A) (Operation.State A)) :=
+  foldl (fun s op => s >>= effect op) s ops
+
+@[simp, grind =] theorem effect_list_nil (s : Except (Operation.Error A) (Operation.State A)) :
+  effect_list [] s = s := by rfl
+
+@[simp, grind =] theorem effect_list_cons (a : A) (ops : List A)
+  (s : Except (Operation.Error A) (Operation.State A)) :
+  effect_list (a :: ops) s = effect_list ops (s >>= effect a) := by rfl
+
+@[simp, grind =] theorem effect_list_append (ops₀ ops₁ : List A)
+  (s : Except (Operation.Error A) (Operation.State A)) :
+  effect_list (ops₀ ++ ops₁) s = effect_list ops₁ (effect_list ops₀ s) := by
   induction ops₀ with
   | nil =>
-    simp
-  | cons b bs ih =>
-    intro h_comm h_concurrent hcompatible
-    simp
-    symm
-    calc
-      _ = ((effect a ▷ effect b) ▷ (foldr effect_comp init (map (fun a => effect a) bs))) s := by rw [effect_comp_assoc]
-      _ = ((effect a ▷ effect b) s >>= (foldr effect_comp init (map (fun a => effect a) bs))) := by rfl
-      _ = ((effect b ▷ effect a) s >>= (foldr effect_comp init (map (fun a => effect a) bs))) := by
-        rw [h_comm a b] <;> try grind [hb_concurrent]
-        simp [hb_concurrent] at *
-        grind
-    rw [ih]
-    . rw [←effect_comp_assoc]
-      have h_effect_b_effect_a_comm : effect b ▷ effect a = effect a ▷ effect b := by
-        ext s
-        apply h_comm
-        . simp
-        . simp
-        . apply h_concurrent; simp
-      rw [h_effect_b_effect_a_comm]
-      rw [effect_comp_assoc]
-    . intros x y h_x_mem h_y_mem
-      apply h_comm
-      . simp at *
-        right; assumption
-      . simp at *
-        right; assumption
-    . intros; apply h_concurrent; simp; right; assumption
+    simp [effect_list]
+  | cons a ops₀ ih =>
+    simp [effect_list]
+
+theorem effect_list_ok_init_ok (ops : List A) (h : effect_list ops s = Except.ok s') :
+  ∃u, s = Except.ok u := by
+  induction ops generalizing s with
+  | nil =>
+    use s'; grind
+  | cons a ops ih =>
+    simp at *
+    apply ih at h
+    obtain ⟨ u, h_s_eq ⟩ := h
+    apply Except.bind_eq_ok_exist at h_s_eq
+    grind
+
+theorem Except.ok_bind {α β ε : Type} (x : α) (f : α -> Except β ε) :
+  (do
+    let x <- Except.ok x
+    f x) = f x := by eq_refl
+
+theorem hb_concurrent_foldr :
+  concurrent_commutative (hb := hb) (ops₀ ++ a :: ops₁) →
+  (∀ x ∈ ops₁, hb_concurrent hb x a) →
+  hb_consistent hb (ops₀ ++ a :: ops₁) →
+  hbClosed hb (ops₀ ++ a :: ops₁) →
+  IdNoDup (ops₀ ++ a :: ops₁) →
+  effect_list ops₁
+    (effect_list ops₀ (Except.ok Operation.init) >>= effect a) = Except.ok s →
+  effect_list ops₁
+    (effect_list ops₀ (Except.ok Operation.init)) >>= effect a = Except.ok s := by
+  induction ops₁ generalizing ops₀ with
+  | nil =>
+    simp [effect_list]
+  | cons b ops₁ ih =>
+    intro h_comm h_concurrent h_consistent h_closed h_no_dup heq
+    simp at *
+    have ⟨ s', h ⟩ : ∃ s, (effect_list ops₀ (Except.ok Operation.init) >>= fun x => effect a x >>= effect b) = Except.ok s := by
+      apply effect_list_ok_init_ok
+      assumption
+    obtain ⟨ u, h_effects_eq, h_effect_b_eq ⟩ := Except.bind_eq_ok_exist h
+    have hba : (effect b u >>= effect a) = Except.ok s' := by
+      apply h_comm a b u s'
+      . simp
+      . simp
+      . sorry
+      . sorry
+      . sorry
+      . assumption
+    have ⟨ sb, h_sb ⟩ : ∃ sb, effect b u = Except.ok sb := by
+      apply Except.bind_eq_ok_exist at hba
+      grind
+    rw [h_effects_eq] at heq |-
+    rw [Except.ok_bind, h_effect_b_eq, ←hba] at heq
+    have heq' : effect_list ops₁ (effect b u >>= effect a) = effect_list ops₁ (effect_list (ops₀ ++ [b]) (Except.ok Operation.init) >>= effect a) := by
+      simp
+      rw [h_effects_eq]; rfl
+    rw [heq'] at heq
+    apply ih at heq
+    . simp at heq
+      rw [h_effects_eq] at heq
+      assumption
+    . sorry
+    . grind
+    . sorry
+    . sorry
+    . sorry
 
 theorem effect_comp_apply {op1 op2 : Effect (A := A)} {s : Operation.State A} :
   effect_comp op1 op2 s = op1 s >>= op2 := by
   rfl
 
-theorem hb_consistent_effect_convergent (ops₀ ops₁ : List A) (init : Effect) s
+theorem hb_consistent_effect_convergent (ops₀ ops₁ : List A)
   (h_consistent₀ : hb_consistent hb ops₀)
   (h_consistent₁ : hb_consistent hb ops₁)
-  (hcompatible₀ : compatibleOps hb s ops₀)
-  (hcompatible₁ : compatibleOps hb s ops₁)
-  (h_commutative : concurrent_commutative hb ops₀)
-  (no_dup₀ : ops₀.Nodup) (no_dup₁ : ops₁.Nodup) :
+  (h_commutative : concurrent_commutative (hb := hb) ops₀)
+  (no_dup₀ : IdNoDup ops₀) (no_dup₁ : IdNoDup ops₁) :
   (∀ a, a ∈ ops₀ ↔ a ∈ ops₁) →
-  (ops₀.map (fun a => effect a) |> List.foldr effect_comp init) s =
-  (ops₁.map (fun a => effect a) |> List.foldr effect_comp init) s :=
+  effect_list ops₀ (Except.ok Operation.init) = Except.ok s →
+  effect_list ops₁ (Except.ok Operation.init) = Except.ok s :=
 by
-  induction ops₀ generalizing ops₁ s with
+  induction ops₁ using List.reverseRecOn generalizing ops₀ s with
   | nil =>
-    intros h_mem
-    have ops₁_eq_nil : ops₁ = [] := by
-      cases ops₁ with
+    intros h_mem hops₀
+    have ops₀_eq_nil : ops₀ = [] := by
+      cases ops₀ with
       | nil => rfl
-      | cons a ops₁ =>
+      | cons a ops₀ =>
         specialize h_mem a
         simp at h_mem
-    rw [ops₁_eq_nil]
-  | cons a ops₀ ih =>
-    intros h_mem
-    cases ops₁ with
-    | nil =>
-      specialize h_mem a
-      simp at h_mem
-    | cons b ops₁ =>
+    grind
+  | append_singleton ops₁ b ih =>
+    intros h_mem hops₀
+    cases List.eq_nil_or_concat' ops₀ with
+    | inl h =>
+      subst h; simp at h_mem; grind
+    | inr h =>
+      replace ⟨ ops₀, a, h ⟩ := h; subst h
       by_cases h_eq : a = b
       . -- Case a = b
-        simp [effect_comp]
-        rw [h_eq]
-        have (eq := hx) x := effect b s; rw [<-hx]
-        cases x with
-        | error e => rfl
-        | ok x =>
-          simp [bind, Except.bind.eq_2]
-          apply ih
-          . apply hb_consistent_tail hb a ops₀ h_consistent₀
-          . apply hb_consistent_tail hb b ops₁ h_consistent₁
-          . cases hcompatible₀; grind
-          . cases hcompatible₁; grind
-          . intros a b h_a_mem h_b_mem h_concurrent
-            apply h_commutative
-            . simp; right; assumption
-            . simp; right; assumption
-            . assumption
-          . simp at no_dup₀
-            obtain ⟨ h_no_dup₀ ⟩ := no_dup₀
-            assumption
-          . simp at no_dup₁
-            obtain ⟨ h_no_dup₁ ⟩ := no_dup₁
-            assumption
-          . subst h_eq
-            apply List.no_dup_cons_eq _ h_mem no_dup₀ no_dup₁
+        simp at hops₀ |-
+        have ⟨ u, h_effects_eq, h_effect_b_eq ⟩ := Except.bind_eq_ok_exist hops₀
+        rw [←h_eq, ih (ops₀ := ops₀) (s := u)]
+        . assumption
+        . apply hb_consistent_sublist _ h_consistent₀; grind
+        . apply hb_consistent_sublist _ h_consistent₁; grind
+        . grind [concurrent_commutative]
+        . grind [IdNoDup]
+        . grind [IdNoDup]
+        . subst h_eq
+          intros x
+          have h := h_mem x
+          simp at h
+          sorry
+        . assumption
       . -- Case a ≠ b
-        have ⟨ ops₁_first, ops₁_last, h_ops₁_eq ⟩ : ∃ ops₁_first ops₁_last, ops₁ = ops₁_first ++ a :: ops₁_last := by
-          have h_a_mem_ops₁ : a ∈ ops₁ := by
-            specialize h_mem a
+        have ⟨ ops₀_first, ops₀_last, h_ops₀_eq ⟩ : ∃ ops₀_first ops₀_last, ops₀ = ops₀_first ++ b :: ops₀_last := by
+          have h_a_mem_ops₀ : b ∈ ops₀ := by
+            specialize h_mem b
             simp at h_mem
-            cases h_mem with
-            | inl h_eq' =>
-              subst h_eq'
-              contradiction
-            | inr h_mem' =>
-              assumption
-          rw [List.mem_iff_append] at h_a_mem_ops₁
+            grind
+          rw [List.mem_iff_append] at h_a_mem_ops₀
           assumption
-        rw [h_ops₁_eq]
-        simp
-        have h_a_concurrent_op₁_first : ∀ x, x ∈ b :: ops₁_first → hb_concurrent hb x a := by
-          intros x h_mem_ops₁_first
-          constructor
-          . cases h_consistent₀ with
-            | cons _ _ h_consistent_tail h_no_lt =>
-              apply h_no_lt
-              have h_x_in_ops1 : x ∈ b :: ops₁ := by
-                rw [h_ops₁_eq]
-                rw [<-List.cons_append]
-                apply List.mem_append_left
-                assumption
-              have x_neq_a : x ≠ a := by
-                rw [h_ops₁_eq] at no_dup₁
-                have h_eq' : (b :: (ops₁_first ++ a :: ops₁_last)) = ((b :: ops₁_first) ++ a :: ops₁_last) := by
-                  simp
-                rw [h_eq'] at no_dup₁
-                rw [List.nodup_append] at no_dup₁
-                obtain ⟨ _, _, h_not_a_mem ⟩ := no_dup₁
-                apply h_not_a_mem
-                . assumption
-                . simp
-              rw [←h_mem] at h_x_in_ops1
-              simp at h_x_in_ops1
-              cases h_x_in_ops1 with
-              | inl h_eq' =>
-                contradiction
-              | inr h_mem' =>
-                assumption
-          . apply hb_consistent_concurrent hb a (b :: ops₁_first) ops₁_last
-            . rw [h_ops₁_eq] at h_consistent₁
-              assumption
-            . assumption
-        subst h_ops₁_eq
+        rw [h_ops₀_eq] at hops₀
+        simp at hops₀ |-
+        have h_a_concurrent_ops₀_last : ∀ x, x ∈ ops₀_last → hb_concurrent hb x b := by
+          sorry
+          -- intros x h_mem_ops₀_last
+          -- constructor
+          -- . cases h_consistent₀ with
+          --   | cons _ _ h_consistent_tail h_no_lt =>
+          --     apply h_no_lt
+          --     have h_x_in_ops1 : x ∈ b :: ops₁ := by
+          --       rw [h_ops₁_eq]
+          --       rw [<-List.cons_append]
+          --       apply List.mem_append_left
+          --       assumption
+          --     have x_neq_a : x ≠ a := by
+          --       rw [h_ops₁_eq] at no_dup₁
+          --       have h_eq' : (b :: (ops₁_first ++ a :: ops₁_last)) = ((b :: ops₁_first) ++ a :: ops₁_last) := by
+          --         simp
+          --       rw [h_eq'] at no_dup₁
+          --       rw [List.nodup_append] at no_dup₁
+          --       obtain ⟨ _, _, h_not_a_mem ⟩ := no_dup₁
+          --       apply h_not_a_mem
+          --       . assumption
+          --       . simp
+          --     rw [←h_mem] at h_x_in_ops1
+          --     simp at h_x_in_ops1
+          --     cases h_x_in_ops1 with
+          --     | inl h_eq' =>
+          --       contradiction
+          --     | inr h_mem' =>
+          --       assumption
+          -- . apply hb_consistent_concurrent hb a (b :: ops₁_first) ops₁_last
+          --   . rw [h_ops₁_eq] at h_consistent₁
+          --     assumption
+          --   . assumption
+        subst h_ops₀_eq
+        have heq : effect_list ops₀_last (effect_list ops₀_first (Except.ok Operation.init) >>= effect b) =
+          effect_list ops₀_last (effect_list ops₀_first (Except.ok Operation.init)) >>= effect b := by
+          have ⟨ s', ⟨ h, heq ⟩  ⟩ := Except.bind_eq_ok_exist hops₀
+          rw [h]
+          apply hb_concurrent_foldr (hb := hb) at h
+          rw [←h]
+          . sorry
+          . sorry
+          . sorry
+          . sorry
+          . sorry
+        rw [heq] at hops₀
+        replace heq : effect_list ops₀_last (effect_list ops₀_first (Except.ok Operation.init)) >>= effect b >>= effect a =
+          effect_list ops₀_last (effect_list ops₀_first (Except.ok Operation.init)) >>= effect a >>= effect b := by
+          have ⟨ s', ⟨ h, heq ⟩  ⟩ := Except.bind_eq_ok_exist hops₀
+          have ⟨ s'', h_effects_eq, h_effect_a_eq ⟩ := Except.bind_eq_ok_exist h
+          rw [h_effects_eq] at hops₀ |-
+          rw [hops₀]
+          apply h_commutative b a at hops₀
+          rw [Except.ok_bind, hops₀]
+          . simp
+          . simp
+          . sorry
+          . sorry
+          . sorry
+        rw [heq] at hops₀
+        replace heq : effect_list ops₀_last (effect_list ops₀_first (Except.ok Operation.init)) >>= effect a =
+          effect_list ops₁ (Except.ok Operation.init) := by
+          have ⟨ s', ⟨ h, heq ⟩  ⟩ := Except.bind_eq_ok_exist hops₀
+          have h := ih (ops₀ := ops₀_first ++ ops₀_last ++ [a]) (s := s') (by sorry) (by sorry) (by sorry) (by sorry) (by sorry)
+            (by sorry) (by simp; assumption)
+          grind
+        rw [heq] at hops₀
+        rw [<-hops₀]
+
         -- Here, we have ops₁ = ops₁_first ++ a :: ops₁_last and a || ops₁_first
-        have h_concurrent : concurrent_commutative hb (ops₁_first ++ a :: ops₁_last) := by
-          intros c d h_c_mem h_d_mem h_concurrent
-          simp at h_c_mem h_d_mem
-          apply h_commutative c d _ _ h_concurrent
-          . rw [h_mem]; simp
-            right; assumption
-          . rw [h_mem]; simp
-            right; assumption
-        have h_a_b_concurrent : hb_concurrent hb a b := by
-          rw [hb_concurrent_symm]
-          apply h_a_concurrent_op₁_first
-          simp
-        have h_a_concurrent_op₁_first : ∀ x, x ∈ ops₁_first → hb_concurrent hb x a := by
-          intros; apply h_a_concurrent_op₁_first; simp; right; assumption
-        rw [hb_concurrent_foldr hb h_concurrent h_a_concurrent_op₁_first]
-        rw [<-effect_comp_assoc]
-        have heq :
-          ((effect b ▷ effect a) ▷ foldr effect_comp (foldr effect_comp init (map (fun a => effect a) ops₁_last))
-            (map (fun a => effect a) ops₁_first)) s =
-          ((effect b ▷ effect a) s) >>= foldr effect_comp (foldr effect_comp init (map (fun a => effect a) ops₁_last))
-            (map (fun a => effect a) ops₁_first) := by
-          simp [effect_comp]
-        rw [heq, h_commutative b a]
-        . have heq :
-            (effect a ▷ effect b) s >>=
-              foldr effect_comp (foldr effect_comp init (map (fun a => effect a) ops₁_last)) (map (fun a => effect a) ops₁_first) =
-            ((effect a ▷ effect b) ▷ foldr effect_comp (foldr effect_comp init (map (fun a => effect a) ops₁_last))
-              (map (fun a => effect a) ops₁_first)) s := by
-            simp [effect_comp]
-          rw [heq]
-          rw [effect_comp_assoc]
-          rw [effect_comp_apply]
-          rw [effect_comp_apply]
-          cases heq : effect a s with
-          | error e => rfl
-          | ok s' =>
-            simp [bind, Except.bind.eq_2]
-            rw [ih (b :: ops₁_first ++ ops₁_last)]
-            . simp
-            . cases h_consistent₀
-              assumption
-            . apply hb_consistent_sublist _ h_consistent₁
-              simp
-            . cases hcompatible₀; grind
-            . cases hcompatible₁
+        -- have h_concurrent : concurrent_commutative (ops₀_first ++ a :: ops₀_last) := by
+        --   intros c d h_c_mem h_d_mem h_concurrent
+        --   simp at h_c_mem h_d_mem
+        --   apply h_commutative c d _ _ h_concurrent
+        --   . rw [h_mem]; simp
+        --     right; assumption
+        --   . rw [h_mem]; simp
+        --     right; assumption
+        -- have h_a_b_concurrent : hb_concurrent hb a b := by
+        --   rw [hb_concurrent_symm]
+        --   apply h_a_concurrent_op₁_first
+        --   simp
+        -- have h_a_concurrent_op₁_first : ∀ x, x ∈ ops₁_first → hb_concurrent hb x a := by
+        --   intros; apply h_a_concurrent_op₁_first; simp; right; assumption
+        -- rw [hb_concurrent_foldr h_concurrent h_a_concurrent_op₁_first]
+        -- rw [<-effect_comp_assoc]
+        -- have heq :
+        --   ((effect b ▷ effect a) ▷ foldr effect_comp (foldr effect_comp init (map (fun a => effect a) ops₁_last))
+        --     (map (fun a => effect a) ops₁_first)) s =
+        --   ((effect b ▷ effect a) s) >>= foldr effect_comp (foldr effect_comp init (map (fun a => effect a) ops₁_last))
+        --     (map (fun a => effect a) ops₁_first) := by
+        --   simp [effect_comp]
+        -- rw [heq, h_commutative b a]
+        -- . have heq :
+        --     (effect a ▷ effect b) s >>=
+        --       foldr effect_comp (foldr effect_comp init (map (fun a => effect a) ops₁_last)) (map (fun a => effect a) ops₁_first) =
+        --     ((effect a ▷ effect b) ▷ foldr effect_comp (foldr effect_comp init (map (fun a => effect a) ops₁_last))
+        --       (map (fun a => effect a) ops₁_first)) s := by
+        --     simp [effect_comp]
+        --   rw [heq]
+        --   rw [effect_comp_assoc]
+        --   rw [effect_comp_apply]
+        --   rw [effect_comp_apply]
+        --   cases heq : effect a s with
+        --   | error e => rfl
+        --   | ok s' =>
+        --     simp [bind, Except.bind.eq_2]
+        --     rw [ih (b :: ops₁_first ++ ops₁_last)]
+        --     . simp
+        --     . cases h_consistent₀
+        --       assumption
+        --     . apply hb_consistent_sublist _ h_consistent₁
+        --       simp
+        --     . cases hcompatible₀; grind
+        --     . cases hcompatible₁
 
-            . intros x y h_x_mem h_ey_mem h_concurrent
-              apply h_commutative
-              simp; right; assumption
-              simp; right; assumption
-              assumption
-            . simp at no_dup₀
-              obtain ⟨ ⟩ := no_dup₀
-              assumption
-            . apply Nodup.sublist _ no_dup₁
-              simp
-            -- . intros op h_op_mem
-            --   obtain ⟨ ops', hops' ⟩ := h_compatible op (by simp [h_op_mem])
-            --   use ops' ++ [a]
-            --   sorry
-            . intros x
-              constructor
-              . intro h_mem₀
-                have h_mem₀_cons : x ∈ a :: ops₀ := by
-                  simp; right; assumption
-                rw [h_mem] at h_mem₀_cons
-                simp at *
-                rcases h_mem₀_cons with h_eq' | ⟨ h | ⟨ h | h ⟩ ⟩
-                . left; assumption
-                . right; left; assumption
-                . subst h; obtain ⟨ h_eq'', _ ⟩ := no_dup₀
-                  contradiction
-                . right; right; assumption
-              . grind
-        . rw [h_mem]
-          simp
-        . simp
-        . simp [hb_concurrent] at *
-          obtain ⟨ h_not_le_ab, h_not_le_ba ⟩ := h_a_b_concurrent
-          constructor <;> assumption
-        . cases hcompatible₁; grind
-        . cases hcompatible₀; grind
+        --     . intros x y h_x_mem h_ey_mem h_concurrent
+        --       apply h_commutative
+        --       simp; right; assumption
+        --       simp; right; assumption
+        --       assumption
+        --     . simp at no_dup₀
+        --       obtain ⟨ ⟩ := no_dup₀
+        --       assumption
+        --     . apply Nodup.sublist _ no_dup₁
+        --       simp
+        --     -- . intros op h_op_mem
+        --     --   obtain ⟨ ops', hops' ⟩ := h_compatible op (by simp [h_op_mem])
+        --     --   use ops' ++ [a]
+        --     --   sorry
+        --     . intros x
+        --       constructor
+        --       . intro h_mem₀
+        --         have h_mem₀_cons : x ∈ a :: ops₀ := by
+        --           simp; right; assumption
+        --         rw [h_mem] at h_mem₀_cons
+        --         simp at *
+        --         rcases h_mem₀_cons with h_eq' | ⟨ h | ⟨ h | h ⟩ ⟩
+        --         . left; assumption
+        --         . right; left; assumption
+        --         . subst h; obtain ⟨ h_eq'', _ ⟩ := no_dup₀
+        --           contradiction
+        --         . right; right; assumption
+        --       . grind
+        -- . rw [h_mem]
+        --   simp
+        -- . simp
+        -- . simp [hb_concurrent] at *
+        --   obtain ⟨ h_not_le_ab, h_not_le_ba ⟩ := h_a_b_concurrent
+        --   constructor <;> assumption
+        -- . cases hcompatible₁; grind
+        -- . cases hcompatible₀; grind
 
-end CausalOrder
+end commutativity
